Interop: Switch to FStar.Buffer

src/test/interop/Interop.fst
@@ -9,7 +9,8 @@ module Interop
 module List = FStar.List.Tot.Base
 
 module HS = FStar.Monotonic.HyperStack
-module P = FStar.Pointer.Base
+// module P = FStar.Pointer.Base
+module B = FStar.Buffer
 open Machine
 
 open Vale_Sem
@@ -17,7 +18,11 @@ open Vale_Sem
 let op_String_Access = Map.sel
 let op_String_Assignment = Map.upd
 
-let sub l i = (UInt32.v l) - i
+let sub l i = l - i
+
+(**
+
+TODO : This was the more generic version taking a variable number of parameters
 
 (* Takes a Hyperstack and a buffer, and updates a low-level Vale heap
    with the contents of the buffer *)
@@ -85,54 +90,56 @@ let up_mem_list heap buffers mem =
     | a :: q -> aux q (reconstruct_buf a accu_mem heap) heap
   in aux buffers mem heap
 
-let rec write_vale_mem contents (length:UInt32.t{UInt32.v length = FStar.Seq.Base.length contents}) addr (i:nat{i <= UInt32.v length}) 
+**)
+
+let rec write_vale_mem contents (length:nat{length = FStar.Seq.Base.length contents}) addr (i:nat{i <= length}) 
       (curr_heap:Vale_Sem.heap{forall j. 0 <= j /\ j < i ==> curr_heap.[addr + j] == Seq.index contents j}) : GTot Vale_Sem.heap (decreases %[sub length i]) =
-    if i >= (UInt32.v length) then curr_heap
+    if i >= length then curr_heap
     else
       write_vale_mem contents length addr (i+1) (curr_heap.[addr + i] <- FStar.Seq.index contents i)
 
-let rec frame_write_vale_mem contents (length:UInt32.t{UInt32.v length = FStar.Seq.Base.length contents}) addr (i:nat{i <= UInt32.v length}) 
+let rec frame_write_vale_mem contents (length:nat{length = FStar.Seq.Base.length contents}) addr (i:nat{i <= length}) 
       (curr_heap:Vale_Sem.heap{forall j. 0 <= j /\ j < i ==> curr_heap.[addr + j] == Seq.index contents j}) : Lemma
       (requires True)
       (ensures (let new_heap = write_vale_mem contents length addr i curr_heap in
-      forall j. j < addr \/ j >= addr + UInt32.v length ==> curr_heap.[j] == new_heap.[j]))
+      forall j. j < addr \/ j >= addr + length ==> curr_heap.[j] == new_heap.[j]))
       (decreases %[sub length i])=
-      if i >= (UInt32.v length) then ()
+      if i >= length then ()
       else frame_write_vale_mem contents length addr (i+1) (curr_heap.[addr+i] <- Seq.index contents i)
 
-let rec load_store_write_vale_mem contents (length:UInt32.t{UInt32.v length = FStar.Seq.Base.length contents}) addr (i:nat{i <= UInt32.v length}) 
+let rec load_store_write_vale_mem contents (length:nat{length = FStar.Seq.Base.length contents}) addr (i:nat{i <= length}) 
       (curr_heap:Vale_Sem.heap{forall j. 0 <= j /\ j < i ==> curr_heap.[addr + j] == Seq.index contents j}) : Lemma
       (requires True)
       (ensures (let new_heap = write_vale_mem contents length addr i curr_heap in
-      forall j. 0 <= j /\ j < UInt32.v length ==> Seq.index contents j == new_heap.[addr + j]))
+      forall j. 0 <= j /\ j < length ==> Seq.index contents j == new_heap.[addr + j]))
       (decreases %[sub length i])=
-      if i >= (UInt32.v length) then ()
+      if i >= length then ()
       else load_store_write_vale_mem contents length addr (i+1)  (curr_heap.[addr+i] <- Seq.index contents i)
 
-val correct_down: HS.mem -> P.(buffer (TBase TUInt8)) -> P.(buffer (TBase TUInt8)) -> Vale_Sem.heap * nat64 * nat64 -> Type0
+val correct_down: HS.mem -> B.buffer UInt8.t -> B.buffer UInt8.t -> Vale_Sem.heap * nat64 * nat64 -> Type0
 let correct_down mem ptr1 ptr2 res =
   let heap, addr1, addr2 = res in
-  let length1 = P.buffer_length ptr1 in
-  let length2 = P.buffer_length ptr2 in
-  let contents1 = P.buffer_as_seq mem ptr1 in
-  let contents2 = P.buffer_as_seq mem ptr2 in
-  (forall i.  0 <= i /\ i < (UInt32.v length1) ==> heap.[addr1 + i] == FStar.Seq.index contents1 i) /\
-  (forall i.  0 <= i /\ i < (UInt32.v length2) ==> heap.[addr2 + i] == FStar.Seq.index contents2 i)
+  let length1 = B.length ptr1 in
+  let length2 = B.length ptr2 in
+  let contents1 = B.as_seq mem ptr1 in
+  let contents2 = B.as_seq mem ptr2 in
+  (forall i.  0 <= i /\ i < length1 ==> heap.[addr1 + i] == FStar.Seq.index contents1 i) /\
+  (forall i.  0 <= i /\ i < length2 ==> heap.[addr2 + i] == FStar.Seq.index contents2 i)
 
 (* Takes a Low* Hyperstack and two buffers (for the moment) and create a vale memory + keep track of the vale addresses *)
-val down_mem: (mem:HS.mem) -> (ptr1:P.(buffer (TBase TUInt8))) -> (ptr2:P.(buffer (TBase TUInt8))) -> GTot (res: (Vale_Sem.heap * nat64 * nat64){correct_down mem ptr1 ptr2 res})
+val down_mem: (mem:HS.mem) -> (ptr1:B.buffer UInt8.t) -> (ptr2:B.buffer UInt8.t) -> GTot (res: (Vale_Sem.heap * nat64 * nat64){correct_down mem ptr1 ptr2 res})
 
 #set-options "--z3rlimit 40"
 
 let down_mem mem ptr1 ptr2 =
   (* Dummy heap *)
   let heap : heap = FStar.Map.const (UInt8.uint_to_t 0) in
-  let length1 = P.buffer_length ptr1 in
-  let length2 = P.buffer_length ptr2 in
-  let contents1 = P.buffer_as_seq mem ptr1 in
-  let contents2 = P.buffer_as_seq mem ptr2 in
+  let length1 = B.length ptr1 in
+  let length2 = B.length ptr2 in
+  let contents1 = B.as_seq mem ptr1 in
+  let contents2 = B.as_seq mem ptr2 in
   let addr1 = 0 in
-  let addr2 = UInt32.v length1 in
+  let addr2 = length1 in
   let heap1 = write_vale_mem contents1 length1 addr1 0 heap in
   load_store_write_vale_mem contents1 length1 addr1 0 heap;
   let heap2 = write_vale_mem contents2 length2 addr2 0 heap1 in
@@ -141,33 +148,37 @@ let down_mem mem ptr1 ptr2 =
   heap2, addr1, addr2
 
 (* Takes a Low* Hyperstack and two buffers (for the moment) and create a vale state *)
-val down: HS.mem -> P.(buffer (TBase TUInt8)) -> P.(buffer (TBase TUInt8)) -> GTot Vale_Sem.state
+val down: HS.mem -> B.buffer UInt8.t -> B.buffer UInt8.t -> GTot Vale_Sem.state
 
 let down mem ptr1 ptr2 =
   let heap, addr1, addr2 = down_mem mem ptr1 ptr2 in
   Vale_Sem.Mkstate true (fun x -> if x = Rax then addr1 else if x = Rbx then addr2 else 0) heap 
 
-val up_mem: Vale_Sem.heap -> P.(buffer (TBase TUInt8)) -> nat64 -> P.(buffer (TBase TUInt8)) -> nat64 -> HS.mem -> GTot HS.mem
+assume val upd: #a:Type -> b:B.buffer a -> (n:nat{n < B.length b}) -> z:a -> h0:HS.mem -> 
+  (h1:HS.mem{B.modifies_1 b h0 h1 /\ B.as_seq h1 b == Seq.upd (B.as_seq h0 b) n z })
+
+let rec write_low_mem heap length addr (buf:(B.buffer UInt8.t){length = B.length buf}) (i:nat{i <= length}) curr_mem : GTot HS.mem (decreases %[sub length i]) = 
+  if i >= length then curr_mem
+  else
+    write_low_mem heap length addr buf (i+1) (upd buf i heap.[addr + i] curr_mem)
+
+val up_mem: Vale_Sem.heap -> (ptr1: B.buffer UInt8.t) -> nat64 -> (ptr2: (B.buffer UInt8.t){B.disjoint ptr1 ptr2}) -> nat64 -> HS.mem -> GTot HS.mem
 
 let up_mem heap ptr1 addr1 ptr2 addr2 mem =
-  let length1 = P.buffer_length ptr1 in
-  let length2 = P.buffer_length ptr2 in
-  let rec aux length addr buf (i:nat{i <= UInt32.v length}) curr_mem : GTot HS.mem (decreases %[sub length i]) =
-    if i >= (UInt32.v length) then curr_mem
-    else
-      aux length addr buf (i+1) (write_buffer buf (UInt32.uint_to_t i) heap.[addr + i] curr_mem)
-  in let mem1 = aux length1 addr1 ptr1 0 mem in
-  let mem2 = aux length2 addr2 ptr2 0 mem in
+  let length1 = B.length ptr1 in
+  let length2 = B.length ptr2 in
+  let mem1 = write_low_mem heap length1 addr1 ptr1 0 mem in
+  let mem2 = write_low_mem heap length2 addr2 ptr2 0 mem in
   mem2
 
-val down_up_identity: (mem:HS.mem) -> (ptr1:P.(buffer (TBase TUInt8))) -> (ptr2:P.(buffer (TBase TUInt8))) -> Lemma 
+val down_up_identity: (mem:HS.mem) -> (ptr1:B.buffer UInt8.t) -> (ptr2:(B.buffer UInt8.t){B.disjoint ptr1 ptr2}) -> Lemma 
   (let heap, addr1, addr2 = down_mem mem ptr1 ptr2 in let new_mem = up_mem heap ptr1 addr1 ptr2 addr2 mem in
     new_mem == mem)
 
 let down_up_identity mem ptr1 ptr2 =
   let heap, addr1, addr2 = down_mem mem ptr1 ptr2 in let new_mem = up_mem heap ptr1 addr1 ptr2 addr2 mem in
-  assume (UInt32.v (P.buffer_length ptr1) > 0); 
-  assert (heap.[addr1] == Seq.index (P.buffer_as_seq mem ptr1) 0);
+  assume (B.length ptr1 > 0); 
+  assert (heap.[addr1] == Seq.index (B.as_seq mem ptr1) 0);
   // assert (Seq.index (P.buffer_as_seq mem ptr1) 0 == Seq.index (P.buffer_as_seq new_mem ptr1) 0);
   // assert (forall i. 0 <= i /\ i < UInt32.v (P.buffer_length ptr1) ==> Seq.index (P.buffer_as_seq mem ptr1) i == Seq.index (P.buffer_as_seq new_mem ptr1) i);
   // assert (P.buffer_as_seq mem ptr1 == P.buffer_as_seq new_mem ptr1);
